Complete the proof that suggestions are safe.

Isabelle2/AbstractMultiPaxosR1Correctness.thy
@@ -18,14 +18,12 @@ subsection {* Automation setup *}
 
 lemmas ioa_defs =
    is_trans_def actions_def trans_def start_def start_s_def
-   externals_def ioa_def asig_def
-
-declare ioa_defs[inv_proofs_defs]
-declare the_ioa_def[inv_proofs_defs]
+   externals_def ioa_def asig_def the_ioa_def
 
 declare propose_def[simp] join_ballot_def[simp] do_vote_def[simp] suggest_def[simp]
-  learn_def[simp] Let_def[simp] if_split[split] if_split_asm[split]
-  acquire_leadership_def[simp]
+  learn_def[simp] Let_def[simp] if_splits[split] acquire_leadership_def[simp]
+
+named_theorems inv_defs
 
 (*  Nitpick config:
 nitpick[no_assms, show_consts, verbose, card 'a = 3, card 'v = 2, card nat = 2, card "'v option" = 3, card "nat option" = 3,
@@ -33,48 +31,52 @@ nitpick[no_assms, show_consts, verbose, card 'a = 3, card 'v = 2, card nat = 2, 
 *)
 method rm_trans_rel_assm = 
   (match premises in P[thin]:"trans_rel ?x ?y ?z" \<Rightarrow> \<open>-\<close>)
-method unfold_to_trans_rel = 
+
+method unfold_to_trans_rel =
   (simp add:is_trans_def the_ioa_def ioa_def trans_def)
 
-
+lemma is_trans_E:
+  "s \<midarrow>a\<midarrow>the_ioa\<longrightarrow> t \<Longrightarrow> trans_rel s a t"
+  by (unfold_to_trans_rel)
+  
 subsection {* Auxiliary invariants *}
 
-definition inv7 where inv7_def[inv_proofs_defs]:
+definition inv7 where inv7_def[inv_defs]:
   "inv7 s \<equiv> \<forall> a . ampr1_state.leader s a \<longrightarrow> leader (ballot s a) = a"
 
 lemma inv7: "invariant the_ioa inv7"
 apply (rule invariantI)
-apply (force simp add:inv_proofs_defs)
+apply (force simp add:inv_defs ioa_defs)
 apply (unfold_to_trans_rel)
 apply (rm_reachable)
 apply ((induct_tac rule:trans_cases, simp); rm_trans_rel_assm)
-apply (auto simp add:inv_proofs_defs)
+apply (auto simp add:inv_defs)
 done
-declare inv7[invs]
+declare inv7
 
-definition inv6 where inv6_def[inv_proofs_defs]:
+definition inv6 where inv6_def[inv_defs]:
   "inv6 s \<equiv> \<forall> a b i . leader b = a \<and> (ballot s a < b \<or> (ballot s a = b \<and> \<not> ampr1_state.leader s a))
     \<longrightarrow> suggestion s i b = None"
 
 lemma inv6: "invariant the_ioa inv6"
 apply (rule invariantI)
-apply (force simp add:inv_proofs_defs)
-apply instantiate_invs_2
+apply (force simp add:inv_defs ioa_defs)
+apply (instantiate_invs_2 invs:inv7)
 apply (unfold_to_trans_rel)
 apply ((induct_tac rule:trans_cases, simp); rm_trans_rel_assm)
-apply (auto simp add:inv_proofs_defs)
+apply (auto simp add:inv_defs)
 done
-declare inv6[invs]
+declare inv6
 
-definition inv1 where inv1_def[inv_proofs_defs]:
+definition inv1 where inv1_def[inv_defs]:
   -- {* acceptors only vote for the suggestion. *}
   "inv1 s \<equiv> \<forall> i a b . let v = vote s i a b in v \<noteq> None \<longrightarrow> v = suggestion s i b"
 
 lemma inv1:
   "invariant the_ioa inv1"
 apply (rule invariantI)
-apply (force simp add:inv_proofs_defs invs)
-apply instantiate_invs_2
+apply (force simp add:inv_defs ioa_defs invs)
+apply (instantiate_invs_2 invs:inv6 inv7)
 apply (unfold_to_trans_rel)
 apply ((induct_tac rule:trans_cases, simp); rm_trans_rel_assm)
               apply (simp_all add:inv1_def)
@@ -82,11 +84,11 @@ apply ((induct_tac rule:trans_cases, simp); rm_trans_rel_assm)
   apply (simp add:inv7_def inv6_def)
   apply force
 done
-declare inv1[invs]
+declare inv1
 
 declare
-  ballot_array.conservative_array_def[inv_proofs_defs]
-  ballot_array.conservative_def[inv_proofs_defs]
+  ballot_array.conservative_array_def[inv_defs]
+  ballot_array.conservative_def[inv_defs]
 
 abbreviation conservative_array where
   "conservative_array s \<equiv>  \<forall> i . ballot_array.conservative_array (vote s i)"
@@ -94,18 +96,18 @@ abbreviation conservative_array where
 lemma conservative: "invariant the_ioa conservative_array"
 proof -
   have "\<And> s . inv1 s \<Longrightarrow> conservative_array s"
-    by (auto simp add:inv_proofs_defs split:option.splits) (metis option.sel)
+    by (auto simp add:inv_defs split:option.splits) (metis option.sel)
   with inv1 show ?thesis  using IOA.invariant_def by blast
 qed
-declare conservative[invs]
+(* declare conservative[invs] *)
 
 lemma trans_imp_prefix_order:
     -- {* This is used to show that safe_at is monotonic *}
   assumes "s \<midarrow>a\<midarrow>the_ioa\<longrightarrow> t"
   shows "is_prefix (ballot s) (ballot t) (vote s i) (vote t i)" using assms
-  apply (simp add:inv_proofs_defs)
+  apply (simp add:inv_defs ioa_defs)
   apply (induct rule:trans_cases)
-  apply (auto simp add:is_prefix_def inv_proofs_defs split:option.split_asm)
+  apply (auto simp add:is_prefix_def inv_defs split:option.split_asm)
 done
 
 abbreviation safe_at where "safe_at s i \<equiv> ballot_array.safe_at quorums (ballot s) (vote s i)"
@@ -116,34 +118,34 @@ lemma safe_mono:
   shows "safe_at t i v b" using assms ballot_array_prefix.safe_at_mono
 by (metis ballot_array_prefix_axioms_def ballot_array_prefix_def quorums_axioms trans_imp_prefix_order) 
 
-definition inv3 where inv3_def[inv_proofs_defs]:
+definition inv3 where inv3_def[inv_defs]:
   "inv3 s \<equiv> \<forall> a b maxs i . onebs s a b = Some maxs \<longrightarrow>
   maxs i = dsa.acc_max (vote s i) a b \<and> ballot s a \<ge> b"
   
 lemma inv3: "invariant the_ioa inv3"
   apply (rule invariantI)
-   apply (force simp add:inv_proofs_defs)
+   apply (force simp add:inv_defs ioa_defs)
   apply instantiate_invs_2
   apply (unfold_to_trans_rel)
   apply ((induct_tac rule:trans_cases, simp); rm_trans_rel_assm;
-      (simp add:inv_proofs_defs  split:option.splits; fail)?)
-   apply (auto simp add:inv_proofs_defs  split:option.splits)[1]
+      (simp add:inv_defs  split:option.splits; fail)?)
+   apply (auto simp add:inv_defs  split:option.splits)[1]
    apply (meson nat_less_le order_trans)
-  apply (auto simp add:inv_proofs_defs dsa.acc_max_def dsa.acc_max_def dsa.a_votes_def 
+  apply (auto simp add:inv_defs dsa.acc_max_def dsa.a_votes_def 
       distributed_safe_at.acc_max_def  split:option.splits)
    apply (smt Collect_cong not_less prod.case_eq_if)
   by (smt Collect_cong not_less prod.case_eq_if)
-declare inv3[invs]
+(* declare inv3[invs] *)
 
 (* nitpick[no_assms, show_consts, verbose, card 'a = 3, card 'v = 2, card nat = 2, card "'v option" = 3, card "nat option" = 3,
     card "('v \<times> nat) option" = 5, card "'v \<times> nat" = 4, card unit = 1, card "('v, 'a) ampr1_state" = 32, card 'l = 1, expect=none]  *)
 
-definition inv5 where inv5_def[inv_proofs_defs]:
+definition inv5 where inv5_def[inv_defs]:
   "inv5 s \<equiv> \<forall> a b f i v b' . onebs s a b = Some f \<and> f i = {(v,b')}
     \<longrightarrow> (vote s i a b' = Some v)"
 lemma inv5:"invariant the_ioa inv5"
   apply (rule invariantI)
-   apply (force simp add:inv_proofs_defs)
+   apply (force simp add:inv_defs ioa_defs)
   apply instantiate_invs_2
   apply (unfold_to_trans_rel)
   apply ((induct_tac rule:trans_cases, simp); rm_trans_rel_assm) oops
@@ -163,21 +165,20 @@ method instantiate_inv uses inv = (
   (* Get rid of the reachability assumption *)
   rm_reachable )
 
-definition inv11 where inv11_def[inv_proofs_defs]:
+definition inv11 where inv11_def[inv_defs]:
   "inv11 s \<equiv> \<forall> a b f i . onebs s a b = Some f \<longrightarrow> f i = dsa.acc_max (vote s i) a b"
 lemma inv11:"invariant the_ioa inv11"
   apply (rule invariantI)
-   apply (simp add:inv_proofs_defs dsa.q_votes_def max_by_key_def)
+   apply (simp add:inv_defs ioa_defs dsa.q_votes_def max_by_key_def)
   apply (instantiate_inv inv:inv3)
   apply (unfold_to_trans_rel)
   apply ((induct_tac rule:trans_cases, simp; rm_trans_rel_assm))
-       apply ((simp_all add:inv_proofs_defs))[2] defer
-     apply ((simp_all add:inv_proofs_defs))[3]
-  apply (simp (no_asm_use) add:inv_proofs_defs)
+       apply ((simp_all add:inv_defs))[2] defer
+     apply ((simp_all add:inv_defs))[3]
+  apply (simp (no_asm_use) add:inv_defs)
   by blast
-declare inv11[invs]
   
-definition inv4 where inv4_def[inv_proofs_defs]:
+definition inv4 where inv4_def[inv_defs]:
   "inv4 s \<equiv> \<forall> i b q . (\<forall> a \<in> q . onebs s a b \<noteq> None) \<longrightarrow>
   (max_vote s i b q = dsa.max_quorum_votes (vote s i) q b)"
 lemma inv4:"invariant the_ioa inv4"
@@ -189,7 +190,7 @@ proof -
     using IOA.invariant_def inv11 by blast 
 qed
 
-definition inv12 where inv12_def[inv_proofs_defs]:
+definition inv12 where inv12_def[inv_defs]:
   "inv12 s \<equiv> \<forall> b i q v . sugg s i b q = Some v \<and> (\<forall> a \<in> q . onebs s a b \<noteq> None) \<and> q \<in> quorums
     \<longrightarrow> dsa.proved_safe_at (ballot s) (vote s i) q b v"
 lemma inv12:"invariant the_ioa inv12"
@@ -219,7 +220,7 @@ proof -
 qed
 
 abbreviation safe where "safe s \<equiv> \<forall> i . ballot_array.safe  quorums (ballot s) (vote s i)"
-declare ballot_array.safe_def[inv_proofs_defs]
+declare ballot_array.safe_def[inv_defs]
 
 lemma aqcuire_leadership_ok:
   fixes a q s t i v safe_at 
@@ -229,7 +230,7 @@ lemma aqcuire_leadership_ok:
   shows "case suggestion t i (ballot t a) of Some v \<Rightarrow> safe_at v | None \<Rightarrow> safe_at v"
 proof -
   let ?b = "ballot s a" 
-  have 3:"?b = ballot t a" using \<open>acquire_leadership a q s t\<close> by (auto simp add:inv_proofs_defs safe_at_def)
+  have 3:"?b = ballot t a" using \<open>acquire_leadership a q s t\<close> by (auto simp add:inv_defs safe_at_def)
   have 1:"q\<in>quorums" and 2:"\<And> a . a \<in> q \<Longrightarrow> ballot s a \<ge> ?b" using \<open>inv3 s\<close> \<open>acquire_leadership a q s t\<close> 
     by (auto simp add:inv3_def) 
   have 4:"vote s = vote t" and 5:"ballot s = ballot t" using \<open>acquire_leadership a q s t\<close> by auto
@@ -268,85 +269,106 @@ proof -
   qed
 qed
 
-definition inv8 where inv8_def[inv_proofs_defs]:
-  "inv8 s \<equiv> \<forall> a i v . let b = ballot s a in
-    ampr1_state.leader s a \<and> suggestion s i b = None \<longrightarrow> safe_at s i v b"
-
 definition inv2 where
   -- {* a suggestion is safe. *}
-  inv2_def[inv_proofs_defs]:
-  "inv2 s \<equiv> \<forall> i b . case suggestion s i b of Some v \<Rightarrow> safe_at s i v b | None \<Rightarrow> True"
+  inv2_def[inv_defs]:
+  "inv2 s \<equiv> safe s \<and> (\<forall> i b . case suggestion s i b of Some v \<Rightarrow> safe_at s i v b 
+  | None \<Rightarrow> (ampr1_state.leader s (leader b) \<and> ballot s (leader b) = b) \<longrightarrow> (\<forall> v . safe_at s i v b))"
 
-lemma inv8_inv2_safe:"invariant the_ioa (\<lambda> s . inv8 s \<and> inv2 s \<and> safe s)" oops
-apply (rule invariantI)
-    apply (force simp add:inv_proofs_defs ballot_array.safe_at_def)
-  apply instantiate_invs_2
-  subgoal premises prems for s t act
-  proof - thm prems
-    note safe_mono[OF prems(2)]
-    thus ?thesis using prems 
-    apply (unfold_to_trans_rel)
-    apply ((induct_tac rule:trans_cases, simp); rm_trans_rel_assm)
-                  apply (auto simp add:inv_proofs_defs split:option.splits)[3]
-            defer
-            apply (auto simp add:inv_proofs_defs split:option.splits)[2]
-            apply (elim conjE)
-        subgoal premises prems for a q
-        proof (rule conjI; (rule conjI)?) thm prems
-          show "safe t" using \<open>safe s\<close> \<open>acquire_leadership a q s t\<close> by (auto simp add:inv_proofs_defs)
-        next
-          show "inv8 t"  proof (auto simp add:inv8_def)
-            fix a2 i v
-            assume a1:"ampr1_state.leader t a2" and a2:"suggestion t i (ballot t a2) = None"
-            show "safe_at t i v (ballot t a2)"
-            proof (cases "a2 = a")
-              case False thus ?thesis using \<open>acquire_leadership a q s t\<close> \<open>inv8 s\<close> \<open>inv7 s\<close> prems(1) a1 a2
-                by (fastforce simp add:inv_proofs_defs)
-            next
-              case True thus ?thesis using aqcuire_leadership_ok \<open>inv3 s\<close> \<open>safe s\<close> \<open>\<forall>i. ballot_array.conservative_array (vote t i)\<close> 
-                \<open>acquire_leadership a q s t\<close> a2 by (metis (mono_tags, lifting) option.case_eq_if)
-            qed
+lemma inv2:"invariant the_ioa inv2"
+  apply (rule invariantI)
+   apply (simp (no_asm_use) add:inv_defs ioa_defs split!:option.splits)
+   apply (simp add: dsa_p.safe_at_0)
+  subgoal premises prems for s t a
+  proof -
+    from prems(3) have 1:"\<And> i v b . safe_at s i v b \<Longrightarrow> safe_at t i v b" using safe_mono by auto
+    show ?thesis using prems
+      apply -
+      apply (instantiate_invs_2 invs:inv4 inv3 inv1 inv7 inv12 conservative)
+      apply (drule is_trans_E)
+      subgoal premises prems
+      proof -
+        have 2:?thesis if "suggestion t = suggestion s" and "ampr1_state.leader t = ampr1_state.leader s"
+          and "ballot t = ballot s" using that 1 \<open>inv1 t\<close> \<open>inv2 s\<close>
+          apply (auto simp add:inv_defs split:option.splits) apply metis by (metis option.distinct(1))
+        show ?thesis using prems
+          apply ((induct_tac rule:trans_cases, simp); rm_trans_rel_assm)
+          subgoal premises prems for c (* propose *)
+          proof -
+            show ?thesis using \<open>inv2 s\<close> \<open>propose c s t\<close> 
+              by (force simp add:inv_defs split!:option.splits) 
           qed
-        next
-          show "inv2 t" proof (auto simp add:inv2_def split:option.splits)
-            fix i b v
-            assume a1:"suggestion t i b = Some v"
-            show "safe_at t i v b"
-            proof (cases "b = ballot s a")
-              case False thus ?thesis using \<open>acquire_leadership a q s t\<close> \<open>inv2 s\<close> prems(1) a1 \<open>inv7 s\<close> 
-                by (auto simp add:inv_proofs_defs split:option.splits)
-            next
-              case True 
-              have 1:"ballot t = ballot s" using \<open>acquire_leadership a q s t\<close> by simp
-              show ?thesis using 1 True aqcuire_leadership_ok[OF \<open>acquire_leadership a q s t\<close> \<open>inv3 s\<close> \<open>safe s\<close> \<open>\<forall>i. ballot_array.conservative_array (vote t i)\<close>, of i]  
-                a1 \<open>inv7 s\<close> by (fastforce simp only:inv7_def Let_def split:option.splits)
-            qed
+          subgoal premises prems for i v (* learn *)
+          proof -
+            show ?thesis using \<open>inv2 s\<close> \<open>learn i v s t\<close> by (simp add:inv_defs)
           qed
-        qed
-        
-      apply (elim conjE)
-      subgoal premises prems for a i v
-      proof (rule conjI; (rule conjI)?) thm prems(12,14,9)
-        show "inv8 t" by (smt ampr1_ioa.do_vote_def ampr1_state.ext_inject ampr1_state.surjective ampr1_state.update_convs(3) inv8_def prems(1) \<open>inv8 s\<close> \<open>do_vote a i v s t\<close>)
-      next
-        show "inv2 t" by (smt prems(1) ampr1_ioa.do_vote_def ampr1_state.ext_inject ampr1_state.surjective ampr1_state.update_convs(3) inv2_def option.case_eq_if \<open>inv2 s\<close>  \<open>do_vote a i v s t\<close>) 
-      next
-        show "safe t" by (smt ampr1_ioa.do_vote_def ampr1_state.ext_inject ampr1_state.surjective ampr1_state.update_convs(3) ballot_array.safe_def inv1_def inv2_def option.case_eq_if prems(1) \<open>do_vote a i v s t\<close> \<open>inv2 s\<close> \<open>inv1 t\<close>) 
+          subgoal premises prems for a b (* join_ballot *) 
+            using \<open>inv2 s\<close> \<open>join_ballot a b s t\<close> 1
+            apply (auto simp add:inv_defs split:option.splits)
+            by (metis option.distinct(1))
+          subgoal premises prems for a i v (* do_vote *)
+            using \<open>do_vote a i v s t\<close> 2 by simp
+          subgoal premises prems for a i b v (* suggest *)
+            apply (auto simp add:inv2_def split:option.split)
+            subgoal using \<open>suggest a i b v s t\<close> \<open>inv2 s\<close> by (simp add:inv2_def)
+            subgoal using \<open>suggest a i b v s t\<close> \<open>inv2 s\<close> by (force simp add:inv2_def split:option.splits)
+            subgoal premises prems2 for i2 b2 w
+            proof (cases "suggestion s i2 b2")
+              case None
+              then show ?thesis using \<open>suggest a i b v s t\<close> \<open>inv2 s\<close> prems2 \<open>inv7 s\<close>
+                apply (cases s, cases t, auto simp add:inv2_def inv7_def split:option.splits)
+                by (metis option.distinct(1))
+            next
+              case (Some v2)
+              then show ?thesis using \<open>suggest a i b v s t\<close> \<open>inv2 s\<close> prems2
+                by (simp add:inv2_def split:option.splits)
+            qed
+            done
+          subgoal premises prems for a q (* acquire_leadership *)
+          proof -
+            have "safe s" using \<open>inv2 s\<close> by (simp add:inv2_def)
+            have "leader (ballot t a) = a" and "q \<in> quorums" using \<open>acquire_leadership a q s t\<close> by auto
+            have "safe t" using \<open>inv2 s\<close> \<open>acquire_leadership a q s t\<close> by (auto simp add:inv2_def)
+            note 3 = aqcuire_leadership_ok[OF \<open>acquire_leadership a q s t\<close> \<open>inv12 s\<close> \<open>inv4 s\<close> \<open>inv3 s\<close> \<open>safe s\<close> \<open>conservative_array s\<close>]
+            show ?thesis using \<open>safe t\<close> 
+              apply (auto simp add:inv2_def split:option.splits)
+              subgoal premises prems2 for i2 b2 v2
+                apply (cases "b2 = ballot t a")
+                subgoal by (metis "3" option.case_eq_if \<open>suggestion t i2 b2 = None\<close>)
+                subgoal premises prems3 using \<open>acquire_leadership a q s t\<close> \<open>inv2 s\<close>
+                  apply (cases s, cases t, auto simp add:inv2_def split:option.splits)
+                  by (metis (no_types, lifting) ampr1_state.select_convs(2) ampr1_state.select_convs(4) ampr1_state.select_convs(6) fun_upd_apply option.distinct(1) prems2(2) prems2(3) prems2(4) prems3)
+                done
+              subgoal for i2 b2 x2 using 3 \<open>acquire_leadership a q s t\<close> \<open>inv2 s\<close> 
+                apply (cases s, cases t, auto simp add:inv2_def fun_upd_def split:option.splits)
+              proof -
+                fix propCmd :: "'b set" and ballota :: "'a \<Rightarrow> nat" and votea :: "nat \<Rightarrow> 'a \<Rightarrow> nat \<Rightarrow> 'b option" and suggestion :: "nat \<Rightarrow> nat \<Rightarrow> 'b option" and onebs :: "'a \<Rightarrow> nat \<Rightarrow> (nat \<Rightarrow> ('b \<times> nat) set) option" and leadera :: "'a \<Rightarrow> bool"
+                assume a1: "\<And>i v. case sugg \<lparr>propCmd = propCmd, ballot = ballota, vote = votea, suggestion = suggestion, onebs = onebs, leader = leadera\<rparr> i (ballota a) q of None \<Rightarrow> safe_at \<lparr>propCmd = propCmd, ballot = ballota, vote = votea, suggestion = \<lambda>i x. if x = ballota a then sugg \<lparr>propCmd = propCmd, ballot = ballota, vote = votea, suggestion = suggestion, onebs = onebs, leader = leadera\<rparr> i (ballota a) q else suggestion i x, onebs = onebs, leader = \<lambda>x. x = a \<or> leadera x\<rparr> i v (ballot \<lparr>propCmd = propCmd, ballot = ballota, vote = votea, suggestion = \<lambda>i x. if x = ballota a then sugg \<lparr>propCmd = propCmd, ballot = ballota, vote = votea, suggestion = suggestion, onebs = onebs, leader = leadera\<rparr> i (ballota a) q else suggestion i x, onebs = onebs, leader = \<lambda>x. x = a \<or> leadera x\<rparr> a) | Some v \<Rightarrow> safe_at \<lparr>propCmd = propCmd, ballot = ballota, vote = votea, suggestion = \<lambda>i x. if x = ballota a then sugg \<lparr>propCmd = propCmd, ballot = ballota, vote = votea, suggestion = suggestion, onebs = onebs, leader = leadera\<rparr> i (ballota a) q else suggestion i x, onebs = onebs, leader = \<lambda>x. x = a \<or> leadera x\<rparr> i v (ballot \<lparr>propCmd = propCmd, ballot = ballota, vote = votea, suggestion = \<lambda>i x. if x = ballota a then sugg \<lparr>propCmd = propCmd, ballot = ballota, vote = votea, suggestion = suggestion, onebs = onebs, leader = leadera\<rparr> i (ballota a) q else suggestion i x, onebs = onebs, leader = \<lambda>x. x = a \<or> leadera x\<rparr> a)"
+                assume "sugg \<lparr>propCmd = propCmd, ballot = ballota, vote = votea, suggestion = suggestion, onebs = onebs, leader = leadera\<rparr> i2 (ballota a) q = Some x2"
+                then have "(case Some x2 of None \<Rightarrow> dsa.safe_at ballota (votea i2) x2 (ballota a) | Some b \<Rightarrow> safe_at \<lparr>propCmd = propCmd, ballot = ballota, vote = votea, suggestion = \<lambda>n na. if na = ballota a then sugg \<lparr>propCmd = propCmd, ballot = ballota, vote = votea, suggestion = suggestion, onebs = onebs, leader = leadera\<rparr> n (ballota a) q else suggestion n na, onebs = onebs, leader = \<lambda>a. a = a \<or> leadera a\<rparr> i2 b (ballot \<lparr>propCmd = propCmd, ballot = ballota, vote = votea, suggestion = \<lambda>n na. if na = ballota a then sugg \<lparr>propCmd = propCmd, ballot = ballota, vote = votea, suggestion = suggestion, onebs = onebs, leader = leadera\<rparr> n (ballota a) q else suggestion n na, onebs = onebs, leader = \<lambda>a. a = a \<or> leadera a\<rparr> a)) = (case sugg \<lparr>propCmd = propCmd, ballot = ballota, vote = votea, suggestion = suggestion, onebs = onebs, leader = leadera\<rparr> i2 (ballota a) q of None \<Rightarrow> safe_at \<lparr>propCmd = propCmd, ballot = ballota, vote = votea, suggestion = \<lambda>n na. if na = ballota a then sugg \<lparr>propCmd = propCmd, ballot = ballota, vote = votea, suggestion = suggestion, onebs = onebs, leader = leadera\<rparr> n (ballota a) q else suggestion n na, onebs = onebs, leader = \<lambda>a. a = a \<or> leadera a\<rparr> i2 x2 (ballot \<lparr>propCmd = propCmd, ballot = ballota, vote = votea, suggestion = \<lambda>n na. if na = ballota a then sugg \<lparr>propCmd = propCmd, ballot = ballota, vote = votea, suggestion = suggestion, onebs = onebs, leader = leadera\<rparr> n (ballota a) q else suggestion n na, onebs = onebs, leader = \<lambda>a. a = a \<or> leadera a\<rparr> a) | Some b \<Rightarrow> safe_at \<lparr>propCmd = propCmd, ballot = ballota, vote = votea, suggestion = \<lambda>n na. if na = ballota a then sugg \<lparr>propCmd = propCmd, ballot = ballota, vote = votea, suggestion = suggestion, onebs = onebs, leader = leadera\<rparr> n (ballota a) q else suggestion n na, onebs = onebs, leader = \<lambda>a. a = a \<or> leadera a\<rparr> i2 b (ballot \<lparr>propCmd = propCmd, ballot = ballota, vote = votea, suggestion = \<lambda>n na. if na = ballota a then sugg \<lparr>propCmd = propCmd, ballot = ballota, vote = votea, suggestion = suggestion, onebs = onebs, leader = leadera\<rparr> n (ballota a) q else suggestion n na, onebs = onebs, leader = \<lambda>a. a = a \<or> leadera a\<rparr> a))"
+                  by simp
+                then show "dsa.safe_at ballota (votea i2) x2 (ballota a)"
+                  using a1
+                  by (smt \<open>sugg \<lparr>propCmd = propCmd, ballot = ballota, vote = votea, suggestion = suggestion, onebs = onebs, leader = leadera\<rparr> i2 (ballota a) q = Some x2\<close> ampr1_state.select_convs(2) ampr1_state.select_convs(3) option.simps(5)) 
+              qed
+              done
+          qed
+          done
       qed
-    done
+      done
   qed
-done
-declare inv8_inv2_safe[invs]
+  done
+declare inv2[invs]
 
 definition inv9 where
-  inv9_def[inv_proofs_defs]:"inv9 s \<equiv> \<forall> i a b . ballot s a < b \<longrightarrow> vote s i a b = None"
+  inv9_def[inv_defs]:"inv9 s \<equiv> \<forall> i a b . ballot s a < b \<longrightarrow> vote s i a b = None"
 
 lemma  inv9:"invariant the_ioa inv9"
 apply (rule invariantI)
-apply (force simp add:inv_proofs_defs)
+apply (force simp add:inv_defs ioa_defs)
   apply (unfold_to_trans_rel)
   apply ((induct_tac rule:trans_cases, simp); rm_reachable; rm_trans_rel_assm;
-      (simp add:inv_proofs_defs; fail)?)
+      (simp add:inv_defs; fail)?)
 done
 declare inv9[invs]
 
@@ -354,30 +376,32 @@ lemma chosen_mono: assumes "chosen s i v" and "s \<midarrow>a\<midarrow>the_ioa\
   shows "chosen t i v" using assms
 apply (unfold_to_trans_rel)
 apply ((induct_tac rule:trans_cases, simp); rm_trans_rel_assm)
-apply (auto simp add:inv_proofs_defs split:option.splits)[3] defer
-apply (auto simp add:inv_proofs_defs split:option.splits)[1]
-apply (cases s, cases t, auto simp add:inv_proofs_defs ballot_array.chosen_def ballot_array.chosen_at_def split:option.splits)
+apply (auto simp add:inv_defs split:option.splits)[3] defer
+apply (auto simp add:inv_defs split:option.splits)[1]
+apply (cases s, cases t, auto simp add:inv_defs ballot_array.chosen_def ballot_array.chosen_at_def split:option.splits)
   by (metis option.distinct(1))
 
-definition inv10 where inv4_def[inv_proofs_defs]:
+(*
+definition inv10 where inv4_def[inv_defs]:
   "inv10 s \<equiv> \<forall> i l . case learned s l i of Some v \<Rightarrow> chosen s i v | None \<Rightarrow> True"
 
 lemma  inv10:"invariant the_ioa inv4"
 apply (rule invariantI)
-apply (force simp add:inv_proofs_defs)
+apply (force simp add:inv_defs)
 apply instantiate_invs_2
 apply (unfold_to_trans_rel)
 apply (induct_tac rule:trans_cases, simp)
-apply (auto simp add:inv_proofs_defs split:option.splits)[3] defer
-apply (auto simp add:inv_proofs_defs split:option.splits)[1]
-apply (insert chosen_mono[simplified inv_proofs_defs])
+apply (auto simp add:inv_defs split:option.splits)[3] defer
+apply (auto simp add:inv_defs split:option.splits)[1]
+apply (insert chosen_mono[simplified inv_defs])
 apply (auto simp add:inv4_def inv5_def  split:option.splits) oops
 by (metis (mono_tags) ampr1_state.select_convs(3) ampr1_state.surjective ampr1_state.update_convs(3) fun_upd_same)
 declare inv4[invs]
 
+
 subsection {* Finally, the proof of agreement. *}
 
-definition agreement where agreement_def[inv_proofs_defs]:
+definition agreement where agreement_def[inv_defs]:
   "agreement s \<equiv> \<forall> i l1 l2 . let v = learned s l1 i; w = learned s l2 i 
     in v \<noteq> None \<and> w \<noteq> None \<longrightarrow> v = w"
 
@@ -386,15 +410,17 @@ proof -
   text {* We prove that @{term inv4} and @{term  safe} imply @{term agreement}. 
     Therefore, since they are invariant, @{term agreement} is invariant} *}
   have "agreement s" if "inv4 s" and "safe s" for s
-  proof (auto simp add:inv_proofs_defs)
+  proof (auto simp add:inv_defs)
     fix i l1 l2 v w
     assume a1:"learned s l1 i = Some v" and a2:"learned s l2 i = Some w"
-    with \<open>inv4 s\<close> have "chosen s i v" and "chosen s i w" by (auto simp add:inv_proofs_defs split:option.splits)
+    with \<open>inv4 s\<close> have "chosen s i v" and "chosen s i w" by (auto simp add:inv_defs split:option.splits)
     with \<open>safe s\<close> show "v = w" by (metis ballot_array_props.intro ballot_array_props.safe_imp_agreement quorums_axioms)
   qed
   thus ?thesis using inv4 inv8_inv2_safe oops by (metis (mono_tags, lifting) IOA.invariant_def)
 qed
     
+*)
+
 end
 
 end
